Add missing proof that new_lock is an m_action

ulib/experimental/Steel.Actions.fst
@@ -494,8 +494,13 @@ let non_alloc_action_to_non_locking_m_action
   : Tot (m_action fp a fp')
 =
   let f_m = non_alloc_action_to_non_locking_pre_m_action fp a fp' f non_alloc in
-  is_m_frame_and_preorder_preserving_intro f_m (fun frame m0 ->
-    admit();
+  let preserves_framing_intro (frame:hprop) (m0:hmem (fp `star` frame))
+    : Lemma (ac_reasoning_for_m_frame_preserving fp frame (locks_invariant Set.empty m0) m0;
+      let (| x, m1 |) = f_m m0 in
+      interp ((fp' x `star` frame) `star` locks_invariant Set.empty m1) (heap_of_mem m1) /\
+      mem_evolves m0 m1
+    )
+    =
     let (| x, m1 |) = f_m m0 in
     assert (interp ((fp `star` frame) `star` locks_invariant Set.empty m0) m0.heap);
     mem_invariant_elim (fp `star` frame) m0;
@@ -513,7 +518,10 @@ let non_alloc_action_to_non_locking_m_action
     assert (interp ((fp' x `star` frame) `star` locks_invariant Set.empty m1) (heap_of_mem m1));
     lock_store_unchanged_respects_preorder m0 m1;
     assert(mem_evolves m0 m1)
-  ) (fun frame m0 f_frame ->
+  in
+  is_m_frame_and_preorder_preserving_intro f_m
+    preserves_framing_intro
+  (fun frame m0 f_frame ->
     ac_reasoning_for_m_frame_preserving fp frame (locks_invariant Set.empty m0) m0;
     let (| x, m1 |) = f_m m0 in
     is_frame_preserving_elim f frame m0.heap f_frame;
@@ -802,7 +810,6 @@ let singleton_heap
   ) in
   h
 
-
 #push-options "--z3rlimit 50 --max_fuel 2 --initial_fuel 2 --initial_ifuel 1 --max_ifuel 1 --warn_error -271"
 let alloc_array_pre_m_action
   (#t: _)
@@ -826,12 +833,12 @@ let alloc_array_pre_m_action
   assert(disjoint m.heap single_h);
   affine_star emp (lock_store_invariant Set.empty m.locks) m.heap;
   assert(interp (lock_store_invariant Set.empty m.locks) (heap_of_mem m));
-  assert(interp (pts_to_array a full_permission (Seq.Base.create (U32.v len) init)) single_h);
-  admit();
-  assert(interp ((pts_to_array a full_permission (Seq.Base.create (U32.v len) init))
-    `star` (lock_store_invariant Set.empty m.locks)) new_h);
+  let h_array = pts_to_array a full_permission (Seq.Base.create (U32.v len) init) in
+  assert(interp h_array single_h);
+  intro_star h_array (lock_store_invariant Set.empty m.locks) single_h (heap_of_mem m);
+  assert(interp (h_array `star` (lock_store_invariant Set.empty m.locks)) new_h);
   let new_m = { m with heap = new_h; ctr = m.ctr +1 } in
-  mem_invariant_intro (pts_to_array a full_permission (Seq.Base.create (U32.v len) init)) new_m;
+  mem_invariant_intro h_array new_m;
   (| a, new_m |)
 #pop-options
 
@@ -1695,35 +1702,65 @@ let equiv_star_left (p q r:hprop)
     (ensures (p `star` q) `equiv` (p `star` r))
   = ()
 
-#push-options "--warn_error -271 --max_fuel 2 --initial_fuel 2 --admit_smt_queries true"
-let new_lock_is_frame_preserving (p:hprop)
-  : Lemma (is_m_frame_and_preorder_preserving (new_lock_pre_m_action p))
-  = let aux (frame:hprop) (m:hmem (p `star` frame))
+let mem_evolves_intro (m:mem) (m1:mem{L.length m1.locks >= L.length m.locks})
+  (same_lock_i: (i:nat{i < L.length m.locks}) ->
+    Lemma (lock_i m.locks i == lock_i m1.locks i))
+  : Lemma (requires L.length m1.locks >= L.length m.locks)
+          (ensures mem_evolves m m1)
+  = Classical.forall_intro same_lock_i
+
+#push-options "--warn_error -271 --fuel 1 --ifuel 0 --z3rlimit 10"
+let new_lock_is_frame_preserving_aux (p:hprop) (frame:hprop) (m:hmem (p `star` frame))
       : Lemma
           (ensures (
+            ac_reasoning_for_m_frame_preserving p frame (locks_invariant Set.empty m) m;
+            (
             let (| x, m1 |) = new_lock_pre_m_action p m in
-            interp (emp `star` frame `star` locks_invariant Set.empty m1) (heap_of_mem m1)))
-          [SMTPat ()]
-      = let (| x, m1 |) = new_lock_pre_m_action p m in
+            interp (emp `star` frame `star` locks_invariant Set.empty m1) (heap_of_mem m1) /\
+            mem_evolves m m1 /\
+            (forall (mp:mprop frame). mp (core_mem m) == mp (core_mem m1))
+            )))
+      = ac_reasoning_for_m_frame_preserving p frame (locks_invariant Set.empty m) m;
+        let (| x, m1 |) = new_lock_pre_m_action p m in
+
+        mem_invariant_elim (p `star` frame) m;
         assert (m1.locks == Available p :: m.locks);
-        assert (locks_invariant Set.empty m1 == (p `star` locks_invariant Set.empty m));
-        assert (interp ((p `star` frame) `star` locks_invariant Set.empty m) (heap_of_mem m));
-        star_associative p frame (locks_invariant Set.empty m);
-        assert (interp (p `star` (frame `star` locks_invariant Set.empty m)) (heap_of_mem m));
-        star_commutative frame (locks_invariant Set.empty m);
-        equiv_star_left p (frame `star` locks_invariant Set.empty m) (locks_invariant Set.empty m `star` frame);
-        assert (interp (p `star` (locks_invariant Set.empty m `star` frame)) (heap_of_mem m));
-        star_associative p (locks_invariant Set.empty m) frame;
-        assert (interp ((p `star` locks_invariant Set.empty m) `star` frame) (heap_of_mem m));
-        assert (interp ((locks_invariant Set.empty m1) `star` frame) (heap_of_mem m));
+        assert (lock_store_invariant Set.empty m1.locks == (p `star` lock_store_invariant Set.empty m.locks));
+        assert (interp ((p `star` frame) `star` lock_store_invariant Set.empty m.locks) (heap_of_mem m));
+        star_associative p frame (lock_store_invariant Set.empty m.locks);
+        assert (interp (p `star` (frame `star` lock_store_invariant Set.empty m.locks)) (heap_of_mem m));
+        star_commutative frame (lock_store_invariant Set.empty m.locks);
+        equiv_star_left p (frame `star` lock_store_invariant Set.empty m.locks) (lock_store_invariant Set.empty m.locks `star` frame);
+        assert (interp (p `star` (lock_store_invariant Set.empty m.locks `star` frame)) (heap_of_mem m));
+        star_associative p (lock_store_invariant Set.empty m.locks) frame;
+        assert (interp ((p `star` lock_store_invariant Set.empty m.locks) `star` frame) (heap_of_mem m));
+        assert (interp ((lock_store_invariant Set.empty m1.locks) `star` frame) (heap_of_mem m));
         assert (heap_of_mem m == heap_of_mem m1);
-        star_commutative (locks_invariant Set.empty m1) frame;
-        assert (interp (frame `star` (locks_invariant Set.empty m1)) (heap_of_mem m1));
-        emp_unit_left (frame `star` (locks_invariant Set.empty m1));
-        assert (interp (emp `star` (frame `star` (locks_invariant Set.empty m1))) (heap_of_mem m1));
-        star_associative emp frame (locks_invariant Set.empty m1)
-    in
-    ()
+        star_commutative (lock_store_invariant Set.empty m1.locks) frame;
+        assert (interp (frame `star` (lock_store_invariant Set.empty m1.locks)) (heap_of_mem m1));
+        emp_unit_left (frame `star` (lock_store_invariant Set.empty m1.locks));
+        assert (interp (emp `star` (frame `star` (lock_store_invariant Set.empty m1.locks))) (heap_of_mem m1));
+        star_associative emp frame (lock_store_invariant Set.empty m1.locks);
+        mem_invariant_intro (emp `star` frame) m1;
+
+        let aux_lock_i (i:nat{i < L.length m.locks})
+          : Lemma (lock_i m.locks i == lock_i m1.locks i)
+          = let (| prefix, li, suffix |) = get_lock m.locks i in
+            let (| prefix', li', suffix' |) = get_lock m1.locks i in
+            L.append_cons_l (Available p) prefix (li::suffix);
+            L.append_length_inv_tail (Available p:: prefix) (li::suffix) prefix' (li'::suffix')
+        in
+
+        mem_evolves_intro m m1 aux_lock_i;
+
+        lift_fp_props_preservation_to_mprops frame m m1
+
+#pop-options
+
+#push-options "--fuel 2 --ifuel 2"
+let new_lock_is_frame_preserving (p:hprop)
+  : Lemma (is_m_frame_and_preorder_preserving (new_lock_pre_m_action p))
+  = Classical.forall_intro_2 (new_lock_is_frame_preserving_aux p)
 #pop-options
 
 let new_lock (p:hprop)
